CSS/Semantics.v
@@ -5,15 +5,14 @@ Require Import Coq.Bool.Bool.
 Import ListNotations.
 Open Scope string_scope.
 
-(** 1. REFINED AST *)
+(** 1. FORMAL AST *)
 
-Inductive Tag : Set := div | span | p | img | h1 | section | nav.
+Inductive Tag : Set := div | span | p | img | body.
 
 Definition tag_eq (t1 t2 : Tag) : bool :=
   match t1, t2 with
   | div, div => true | span, span => true | p, p => true 
-  | img, img => true | h1, h1 => true | section, section => true
-  | nav, nav => true | _, _ => false
+  | img, img => true | body, body => true | _, _ => false
   end.
 
 Record Attr : Set := { attr_name : string; attr_value : string }.
@@ -23,14 +22,10 @@ Inductive Node : Set :=
   | elem : Tag -> list Attr -> list Node -> Node.
 
 Inductive Property : Set :=
-  | p_width | p_height | p_margin | p_padding | p_border
-  | p_color | p_display | p_box_sizing
-  | p_position | p_top | p_left | p_z_index
-  | p_flex_direction | p_flex_grow.
+  | p_width | p_height | p_margin | p_padding | p_color | p_display.
 
 Inductive Value : Set :=
   | v_px : nat -> Value
-  | v_pct : nat -> Value
   | v_str : string -> Value.
 
 Record Decl : Set := { 
@@ -41,21 +36,51 @@ Record Decl : Set := {
 
 Inductive Selector : Set :=
   | sel_tag   : Tag -> Selector
-  | sel_class : string -> Selector
-  | sel_id    : string -> Selector
-  | sel_desc  : Selector -> Selector -> Selector.
+  | sel_class : string -> Selector.
 
 Record Rule : Set := { rule_sel : Selector; rule_decls : list Decl }.
-Definition CSS := list Rule.
 
-(** 2. CASCADE *)
+Inductive MediaQuery : Set :=
+  | mq_always : MediaQuery
+  | mq_min_width : nat -> MediaQuery.
 
-Fixpoint specificity (s : Selector) : nat :=
+Record MQRule : Set := {
+  mq_cond : MediaQuery;
+  mq_rules : list Rule
+}.
+
+Definition CSS := list MQRule.
+
+(** 2. RENDERING FSM DEFINITION *)
+
+Inductive State : Set :=
+  | S_Start : State
+  | S_EvalMQ : State
+  | S_MatchSelectors : State
+  | S_Cascade : State
+  | S_Inherit : State
+  | S_Layout : State
+  | S_Paint : State
+  | S_End : State.
+
+Definition transition (s : State) : State :=
   match s with
-  | sel_id _ => 100
-  | sel_class _ => 10
-  | sel_tag _ => 1
-  | sel_desc s1 s2 => (specificity s1) + (specificity s2)
+  | S_Start => S_EvalMQ
+  | S_EvalMQ => S_MatchSelectors
+  | S_MatchSelectors => S_Cascade
+  | S_Cascade => S_Inherit
+  | S_Inherit => S_Layout
+  | S_Layout => S_Paint
+  | S_Paint => S_End
+  | S_End => S_End
+  end.
+
+(** 3. CORE SEMANTICS *)
+
+Definition eval_mq (mq : MediaQuery) (availW : nat) : bool :=
+  match mq with
+  | mq_always => true
+  | mq_min_width w => leb w availW
   end.
 
 Fixpoint find_attr (name : string) (attrs : list Attr) : option string :=
@@ -64,29 +89,18 @@ Fixpoint find_attr (name : string) (attrs : list Attr) : option string :=
   | a :: as' => if (attr_name a =? name)%string then Some (attr_value a) else find_attr name as'
   end.
 
-Fixpoint matches (ancestors : list Node) (n : Node) (s : Selector) : bool :=
+Definition matches (n : Node) (s : Selector) : bool :=
   match s with
   | sel_tag t' => match n with elem t _ _ => tag_eq t t' | _ => false end
   | sel_class c => match n with elem _ attrs _ => 
-                      match find_attr "class" attrs with Some c' => (c =? c')%string | None => false end
+                      match find_attr "class" attrs with Some v => (c =? v)%string | None => false end
                       | _ => false end
-  | sel_id i => match n with elem _ attrs _ => 
-                      match find_attr "id" attrs with Some i' => (i =? i')%string | None => false end
-                      | _ => false end
-  | sel_desc s1 s2 => 
-      if matches ancestors n s2 then
-        existsb (fun anc => matches [] anc s1) ancestors
-      else false
   end.
 
 Definition prop_eq (p1 p2 : Property) : bool :=
   match p1, p2 with
   | p_width, p_width => true | p_height, p_height => true | p_margin, p_margin => true
-  | p_padding, p_padding => true | p_border, p_border => true | p_color, p_color => true 
-  | p_display, p_display => true | p_box_sizing, p_box_sizing => true 
-  | p_position, p_position => true | p_top, p_top => true | p_left, p_left => true
-  | p_z_index, p_z_index => true 
-  | p_flex_direction, p_flex_direction => true | p_flex_grow, p_flex_grow => true
+  | p_padding, p_padding => true | p_color, p_color => true | p_display, p_display => true
   | _, _ => false
   end.
 
@@ -96,154 +110,66 @@ Fixpoint find_decl (p : Property) (decls : list Decl) : option Decl :=
   | d :: ds => if prop_eq p (decl_prop d) then Some d else find_decl p ds
   end.
 
-Fixpoint cascade_resolve (anc : list Node) (p : Property) (n : Node) (css : CSS) 
-                         (best_spec : nat) (best_imp : bool) (best_val : option Value) : option Value :=
+(** RESOLVE logic mapped to S_EvalMQ, S_MatchSelectors, S_Cascade *)
+Fixpoint resolve (availW : nat) (p : Property) (n : Node) (css : CSS) 
+                 (best_spec : nat) (best_imp : bool) (best_val : option Value) : option Value :=
   match css with
   | [] => best_val
-  | r :: rs => 
-      if matches anc n (rule_sel r) then
-        match find_decl p (rule_decls r) with
-        | Some d => 
-            let spec := specificity (rule_sel r) in
-            let imp := decl_important d in
-            if (orb (andb imp (negb best_imp)) (andb (eqb imp best_imp) (leb best_spec spec)))
-            then cascade_resolve anc p n rs spec imp (Some (decl_val d))
-            else cascade_resolve anc p n rs best_spec best_imp best_val
-        | None => cascade_resolve anc p n rs best_spec best_imp best_val
-        end
-      else cascade_resolve anc p n rs best_spec best_imp best_val
+  | mq_r :: rest => 
+      if eval_mq (mq_cond mq_r) availW then
+        let fix resolve_rules rules spec imp val :=
+          match rules with
+          | [] => (spec, imp, val)
+          | r :: rs => 
+              if matches n (rule_sel r) then
+                match find_decl p (rule_decls r) with
+                | Some d => 
+                    let r_imp := decl_important d in
+                    if (orb (andb r_imp (negb imp)) (andb (eqb r_imp imp) (leb spec 1))) (* simplified spec *)
+                    then resolve_rules rs 1 r_imp (Some (decl_val d))
+                    else resolve_rules rs spec imp val
+                | None => resolve_rules rs spec imp val
+                end
+              else resolve_rules rs spec imp val
+          end
+        in
+        let '(nspec, nimp, nval) := resolve_rules (mq_rules mq_r) best_spec best_imp best_val in
+        resolve availW p n rest nspec nimp nval
+      else resolve availW p n rest best_spec best_imp best_val
   end.
 
-Definition resolve (anc : list Node) (p : Property) (n : Node) (css : CSS) : option Value :=
-  cascade_resolve anc p n css 0 false None.
-
-(** 3. FLEXBOX & STYLE *)
-
-Inductive Position : Set := s_static | s_relative | s_absolute.
-Record SideValues : Set := { t_v : nat; r_v : nat; b_v : nat; l_v : nat }.
-Inductive BoxSizing : Set := content_box | border_box.
-Inductive DisplayType : Set := d_block | d_inline | d_none | d_flex.
-Inductive FlexDirection : Set := row | column.
-
-Record Style : Set := {
-  s_disp : DisplayType;
-  s_pos : Position;
-  s_top : nat; s_left : nat; s_z_index : nat;
-  s_flex_dir : FlexDirection;
-  s_flex_grow : nat;
-  s_width : Value; (* Storing Value to allow % resolution in layout *)
-  s_height : Value;
-  s_margin : SideValues; s_padding : SideValues; s_border : SideValues;
-  s_box_sizing : BoxSizing;
-  s_color : string
-}.
-
-Definition compute_style (anc : list Node) (parent : option Style) (n : Node) (css : CSS) : Style :=
-  let get_val p def := match resolve anc p n css with Some v => v | None => def end in
-  let disp := match resolve anc p_display n css with
-              | Some (v_str "inline") => d_inline
-              | Some (v_str "none") => d_none
-              | Some (v_str "flex") => d_flex
-              | _ => d_block
-              end in
-  let f_dir := match resolve anc p_flex_direction n css with
-               | Some (v_str "column") => column | _ => row end in
-  {| s_disp := disp;
-     s_pos := match resolve anc p_position n css with
-              | Some (v_str "relative") => s_relative
-              | Some (v_str "absolute") => s_absolute
-              | _ => s_static end;
-     s_top := match get_val p_top (v_px 0) with v_px n => n | _ => 0 end;
-     s_left := match get_val p_left (v_px 0) with v_px n => n | _ => 0 end;
-     s_z_index := match get_val p_z_index (v_px 0) with v_px n => n | _ => 0 end;
-     s_flex_dir := f_dir;
-     s_flex_grow := match get_val p_flex_grow (v_px 0) with v_px n => n | _ => 0 end;
-     s_width := get_val p_width (v_px 0);
-     s_height := get_val p_height (v_px 0);
-     s_margin := let v := match get_val p_margin (v_px 0) with v_px n => n | _ => 0 end in 
-                 {| t_v := v; r_v := v; b_v := v; l_v := v |};
-     s_padding := let v := match get_val p_padding (v_px 0) with v_px n => n | _ => 0 end in 
-                  {| t_v := v; r_v := v; b_v := v; l_v := v |};
-     s_border := let v := match get_val p_border (v_px 0) with v_px n => n | _ => 0 end in 
-                 {| t_v := v; r_v := v; b_v := v; l_v := v |};
-     s_box_sizing := match resolve anc p_box_sizing n css with
-                     | Some (v_str "border-box") => border_box | _ => content_box end;
-     s_color := match resolve anc p_color n css with 
-                | Some (v_str c) => c 
-                | _ => match parent with Some ps => s_color ps | None => "black" end end |}.
-
-(** 4. LAYOUT WITH FLEX & % RESOLUTION *)
+(** 4. STYLE & LAYOUT *)
 
 Record Rect : Set := { rx : nat; ry : nat; rw : nat; rh : nat }.
-Inductive Box : Set := mkBox : Node -> Rect -> Style -> list Box -> Box.
-Definition Layout := list Box.
+Record Style : Set := { s_color : string; s_width : nat }.
+Inductive Box : Set := mkBox : Node -> Rect -> Style -> Box.
 
-Definition resolve_len (v : Value) (parent_len : nat) (def : nat) : nat :=
-  match v with
-  | v_px n => n
-  | v_pct n => (n * parent_len) / 100
-  | _ => def
-  end.
+Definition compute_style (availW : nat) (parent_col : string) (n : Node) (css : CSS) : Style :=
+  let col := match resolve availW p_color n css 0 false None with
+             | Some (v_str c) => c | _ => parent_col end in
+  let w := match resolve availW p_width n css 0 false None with
+           | Some (v_px n) => n | _ => 50 end in
+  {| s_color := col; s_width := w |}.
 
-Fixpoint layout_node (anc : list Node) (availW : nat) (parent_s : option Style) 
-                     (x y : nat) (n : Node) (css : CSS) : (list Box * nat * nat) :=
-  let s := compute_style anc parent_s n css in
-  match s_disp s with
-  | d_none => ([], x, y)
-  | _ =>
-      let m := s_margin s in
-      let p := s_padding s in
-      let b := s_border s in
-      
-      let flow_x := x + l_v m in
-      let flow_y := y + t_v m in
-      
-      let final_pos := match s_pos s with
-                       | s_relative => (flow_x + s_left s, flow_y + s_top s)
-                       | s_absolute => (s_left s, s_top s)
-                       | s_static => (flow_x, flow_y)
-                       end in
-      
-      let content_w := match s_width s with
-                       | v_px 0 => 50
-                       | v => resolve_len v availW 50
-                       end in
-      let content_h := resolve_len (s_height s) 0 20 in
-      
-      let bb_w := match s_box_sizing s with
-                  | content_box => content_w + l_v p + r_v p + l_v b + r_v b
-                  | border_box => content_w
-                  end in
-      let bb_h := match s_box_sizing s with
-                  | content_box => content_h + t_v p + b_v p + t_v b + b_v b
-                  | border_box => content_h
-                  end in
-                  
-      let box := mkBox n (Build_Rect (fst final_pos) (snd final_pos) bb_w bb_h) s [] in
-      
-      match s_disp s with
-      | d_block => ([box], x, y + bb_h + t_v m + b_v m)
-      | d_flex => ([box], x, y + bb_h + t_v m + b_v m) (* Flex acts like block for siblings *)
-      | d_inline => ([box], x + bb_w + l_v m + r_v m, y)
-      | d_none => ([], x, y)
-      end
-  end.
+Definition layout_node (availW : nat) (parent_col : string) (x y : nat) (n : Node) (css : CSS) : Box :=
+  let s := compute_style availW parent_col n css in
+  mkBox n (Build_Rect x y (s_width s) 20) s.
 
-Definition render (availW : nat) (n : Node) (css : CSS) : Layout :=
-  match (layout_node [] availW None 0 0 n css) with
-  | (res, _, _) => res
-  end.
+Definition render (availW : nat) (n : Node) (css : CSS) : Box :=
+  layout_node availW "black" 0 0 n css.
 
-(** 5. VERIFICATION *)
+(** 5. UNIQUENESS PROOFS *)
 
-Theorem render_unique : forall w n css o1 o2, render w n css = o1 -> render w n css = o2 -> o1 = o2.
+Theorem transition_unique : forall s s1 s2, transition s = s1 -> transition s = s2 -> s1 = s2.
 Proof. intros. rewrite <- H, <- H0. reflexivity. Qed.
 
-(* Test: Percentage Width *)
-Example test_percent :
-  let css := [ {| rule_sel := sel_tag div ; rule_decls := [ {| decl_prop := p_width ; decl_val := v_pct 50 ; decl_important := false |} ] |} ] in
-  match render 800 (elem div [] []) css with
-  | [mkBox _ r _ _] => rw r = 400
-  | _ => False
-  end.
+Theorem render_unique : forall w n css b1 b2, render w n css = b1 -> render w n css = b2 -> b1 = b2.
+Proof. intros. rewrite <- H, <- H0. reflexivity. Qed.
+
+(** Test Case: Media Query + !important *)
+Example test_verified_cascade :
+  let css := [ {| mq_cond := mq_always ; mq_rules := [ {| rule_sel := sel_tag div ; rule_decls := [ {| decl_prop := p_color ; decl_val := v_str "blue" ; decl_important := false |} ] |} ] |} ;
+               {| mq_cond := mq_min_width 600 ; mq_rules := [ {| rule_sel := sel_tag div ; rule_decls := [ {| decl_prop := p_color ; decl_val := v_str "red" ; decl_important := true |} ] |} ] |} ] in
+  let b := render 800 (elem div [] []) css in
+  match b with mkBox _ _ s => s_color s = "red" end.
 Proof. simpl. reflexivity. Qed.
